OS soundness now includes a trace of events.

progs/io_combine.v
@@ -21,7 +21,7 @@ Notation "' p <- t1 ;; t2" :=
   (ITree.bind t1 (fun x_ => match x_ with p => t2 end))
 (at level 100, t1 at next level, p pattern, right associativity) : itree_scope.
 
-Section ext_safe.
+(*Section ext_safe.
 
   Context {Espec : OracleKind} {OS_state : Type} {etrace : Type}.
   Variable prog : Clight.program.
@@ -91,9 +91,7 @@ Section ext_safe.
        Genv.find_symbol (Genv.globalenv prog) (prog_main prog) = Some b /\
        initial_core  (cl_core_sem (globalenv prog))
            0 m q m' (Vptr b Ptrofs.zero) nil /\
-       forall n,
-        ext_safeN
-             n initial_oracle q m'.
+       forall n, ext_safeN n initial_oracle q m'.
   Proof.
     intros.
     eapply CSHL_Sound.semax_prog_ext_sound, whole_program_sequential_safety_ext in H as (b & q & m' & ? & ? & Hsafe); eauto.
@@ -101,7 +99,221 @@ Section ext_safe.
     eapply dry_safe_ext_safe; eauto.
   Qed.
 
-End ext_safe.
+End ext_safe.*)
+
+Require Import ITree.Interp.Traces.
+Require Import Ensembles.
+
+Section ext_trace.
+
+  Context {cevent : Type -> Type} {J : juicy_ext_spec (itree cevent unit)} {OS_state : Type} {event : Type}.
+  Variable prog : Clight.program.
+  Variable ext_sem : external_function -> list val -> OS_state -> OS_state * option val * list event.
+  Variable inj_mem : mem -> OS_state -> Prop.
+  Variable extr_mem : OS_state -> mem.
+  Notation ge := (globalenv prog).
+
+  Instance Espec : OracleKind := Build_OracleKind (itree cevent unit) J.
+
+  Variable lift_event : event -> {X & (cevent X * X)%type}.
+
+  Fixpoint trace_of_events (t : list event) : @trace cevent unit :=
+    match t with
+    | nil => TEnd
+    | e :: t' =>
+        let (e', r) := projT2 (lift_event e) in
+        TEventResponse e' r (trace_of_events t')
+    end.
+
+  Definition consume_trace (z z' : itree cevent unit) le := let t := trace_of_events le in
+    forall t', is_trace z' t' -> is_trace z (app_trace t t').
+
+(*  Inductive ext_traceN : nat -> list event -> OK_ty -> corestate -> mem -> Prop :=
+  | ext_traceN_0: forall z c m, ext_traceN O [] z c m
+  | ext_traceN_step:
+      forall n t z c m c' m',
+      cl_step ge c m c' m' ->
+      ext_traceN n t z c' m' ->
+      ext_traceN (S n) t z c m
+  | ext_traceN_external:
+      forall n z c m e args,
+      cl_at_external c = Some (e,args) ->
+      forall s s' ret m' t t' n'
+       (Hargsty : Val.has_type_list args (sig_args (ef_sig e)))
+       (Hretty : step_lemmas.has_opttyp ret (sig_res (ef_sig e))),
+       inj_mem m s ->
+       ext_sem e args s = (s', ret, t) ->
+       m' = extr_mem s' ->
+       (n' <= n)%nat ->
+       forall z' c', consume_trace z z' t ->
+       cl_after_external ret c = Some c' ->
+       ext_traceN n' t' z' c' m' ->
+      ext_traceN (S n) (t ++ t') z c m.*)
+
+  Lemma consume_trace_nil : forall z, consume_trace z z nil.
+  Proof.
+    repeat intro; auto.
+  Qed.
+
+  Lemma trace_of_events_app : forall t t', trace_of_events (t ++ t') = app_trace (trace_of_events t) (trace_of_events t').
+  Proof.
+    induction t; auto; simpl; intros.
+    destruct (lift_event a) as (? & ? & ?); simpl.
+    rewrite IHt; auto.
+  Qed.
+
+  Lemma app_trace_assoc : forall {E : Type -> Type} {R : Type} (t t' t'' : @trace E R),
+    app_trace (app_trace t t') t'' = app_trace t (app_trace t' t'').
+  Proof.
+    induction t; auto; simpl; intros.
+    rewrite IHt; auto.
+  Qed.
+
+  Lemma consume_trace_app : forall z z' z'' t t', consume_trace z z' t -> consume_trace z' z'' t' ->
+    consume_trace z z'' (t ++ t').
+  Proof.
+    unfold consume_trace; intros.
+    rewrite trace_of_events_app, app_trace_assoc; auto.
+  Qed.
+
+(*  Theorem ext_trace_correct:
+   forall (initial_oracle: OK_ty) q m n t,
+    ext_traceN n t initial_oracle q m ->
+    exists z', consume_trace initial_oracle z' t.
+  Proof.
+    induction 1.
+    - exists z; repeat intro; auto.
+    - auto.
+    - destruct IHext_traceN as [z'' ?].
+      exists z''.
+      eapply consume_trace_app; eauto.
+  Qed.*)
+
+  Inductive ext_safeN_trace : nat -> Ensemble (list event) -> OK_ty -> corestate -> mem -> Prop :=
+  | ext_safeN_trace_0: forall z c m, ext_safeN_trace O (Empty_set _) z c m
+  | ext_safeN_trace_step:
+      forall n traces z c m c' m',
+      cl_step ge c m c' m' ->
+      ext_safeN_trace n traces z c' m' ->
+      ext_safeN_trace (S n) traces z c m
+  | ext_safeN_trace_external:
+      forall n traces z c m e args,
+      cl_at_external c = Some (e,args) ->
+      (forall s s' ret m' t n'
+         (Hargsty : Val.has_type_list args (sig_args (ef_sig e)))
+         (Hretty : step_lemmas.has_opttyp ret (sig_res (ef_sig e))),
+         inj_mem m s ->
+         ext_sem e args s = (s', ret, t) ->
+         m' = extr_mem s' ->
+         (n' <= n)%nat ->
+         exists traces' z' c', consume_trace z z' t /\
+           cl_after_external ret c = Some c' /\
+           ext_safeN_trace n' traces' z' c' m' /\
+           (forall t', In _ traces' t' -> In _ traces (t ++ t'))) ->
+      (forall t1, In _ traces t1 ->
+        exists s s' ret m' t n', Val.has_type_list args (sig_args (ef_sig e)) /\
+         step_lemmas.has_opttyp ret (sig_res (ef_sig e)) /\
+         inj_mem m s /\ ext_sem e args s = (s', ret, t) /\ m' = extr_mem s' /\
+         (n' <= n)%nat /\ exists traces' z' c', consume_trace z z' t /\
+           cl_after_external ret c = Some c' /\ ext_safeN_trace n' traces' z' c' m' /\
+        exists t', In _ traces' t' /\ t1 = t ++ t') ->
+      ext_safeN_trace (S n) traces z c m.
+
+  Variable dryspec : ext_spec OK_ty.
+  Hypothesis extcalls_correct : forall e w b tl args z m s, ext_spec_pre dryspec e w b tl args z m ->
+    inj_mem m s ->
+    let '(s', ret, t') := ext_sem e args s in
+    exists z', consume_trace z z' t' /\
+    ext_spec_post dryspec e w b (sig_res (ef_sig e)) ret z' (extr_mem s').
+
+  Lemma dry_safe_ext_trace_safe : forall n z q m,
+    step_lemmas.dry_safeN(genv_symb := Clight_sim.genv_symb_injective)
+     (Clight_sim.coresem_extract_cenv (cl_core_sem (globalenv prog)) (prog_comp_env prog)) dryspec
+     (Build_genv (Genv.globalenv prog) (prog_comp_env prog)) n z q m ->
+    exists traces, ext_safeN_trace n traces z q m.
+  Proof.
+    induction n as [n IHn] using lt_wf_ind; intros; inversion H; subst; try contradiction.
+    - eexists; constructor.
+    - edestruct IHn as [traces ?]; eauto; exists traces; econstructor; eauto.
+    - exists (fun t1 => exists s s' ret m' t n', Val.has_type_list args (sig_args (ef_sig e)) /\
+         step_lemmas.has_opttyp ret (sig_res (ef_sig e)) /\
+         inj_mem m s /\ ext_sem e args s = (s', ret, t) /\ m' = extr_mem s' /\
+         (n' <= n0)%nat /\ exists traces' z' c', consume_trace z z' t /\
+           cl_after_external ret q = Some c' /\ ext_safeN_trace n' traces' z' c' m' /\
+        exists t', In _ traces' t' /\ t1 = t ++ t').
+      eapply ext_safeN_trace_external; eauto; intros.
+      eapply extcalls_correct in H1; eauto.
+      rewrite H4 in H1; destruct H1 as (z' & ? & ?).
+      edestruct H2 as (? & ? & Hsafe); eauto.
+      apply IHn in Hsafe as [traces ?]; [|omega].
+      subst; do 4 eexists; eauto; split; eauto; split; eauto.
+      intros; unfold In.
+      do 7 eexists; eauto; split; eauto; split; eauto; split; eauto; split; eauto; split; eauto.
+      do 4 eexists; eauto.
+  Qed.
+
+  Lemma safety_trace:
+   forall {CS: compspecs} (initial_oracle: OK_ty)
+     (dessicate : forall (ef : external_function) jm,
+               ext_spec_type OK_spec ef ->
+               ext_spec_type dryspec ef)
+     (JDE: juicy_dry_ext_spec _ (@JE_spec OK_ty OK_spec) dryspec dessicate)
+     (DME: ext_spec_mem_evolve _ dryspec)
+     V G m,
+     @semax_prog_ext Espec CS prog initial_oracle V G ->
+     Genv.init_mem prog = Some m ->
+     exists b, exists q, exists m',
+       Genv.find_symbol (Genv.globalenv prog) (prog_main prog) = Some b /\
+       initial_core  (cl_core_sem (globalenv prog))
+           0 m q m' (Vptr b Ptrofs.zero) nil /\
+       forall n, exists traces, ext_safeN_trace n traces initial_oracle q m'.
+  Proof.
+    intros.
+    eapply CSHL_Sound.semax_prog_ext_sound, whole_program_sequential_safety_ext in H as (b & q & m' & ? & ? & Hsafe); eauto.
+    do 4 eexists; eauto; split; eauto; intro n.
+    eapply dry_safe_ext_trace_safe; eauto.
+  Qed.
+
+  Lemma trace_correct:
+   forall n (z: OK_ty) q m traces t,
+    ext_safeN_trace n traces z q m ->
+    In _ traces t ->
+    exists z', consume_trace z z' t.
+  Proof.
+    induction n as [n IHn] using lt_wf_ind; intros; inversion H; subst.
+    - inversion H0.
+    - eauto.
+    - destruct (H3 _ H0) as (s & s' & ret & m' & t1 & n' & ? & ? & ? & ? & ? & ? & traces' & z' & c' & ? & ? & ? & ? & ? & ?).
+      edestruct (IHn n') as [z'' ?]; eauto; [omega|].
+      subst; eexists; eapply consume_trace_app; eauto.
+  Qed.
+
+  Theorem OS_soundness:
+   forall {CS: compspecs} (initial_oracle: OK_ty)
+     (dessicate : forall (ef : external_function) jm,
+               ext_spec_type OK_spec ef ->
+               ext_spec_type dryspec ef)
+     (JDE: juicy_dry_ext_spec _ (@JE_spec OK_ty OK_spec) dryspec dessicate)
+     (DME: ext_spec_mem_evolve _ dryspec)
+     V G m,
+     @semax_prog_ext Espec CS prog initial_oracle V G ->
+     Genv.init_mem prog = Some m ->
+     exists b, exists q, exists m',
+       Genv.find_symbol (Genv.globalenv prog) (prog_main prog) = Some b /\
+       initial_core  (cl_core_sem (globalenv prog))
+           0 m q m' (Vptr b Ptrofs.zero) nil /\
+       forall n, exists traces, ext_safeN_trace n traces initial_oracle q m' /\
+         forall t, In _ traces t -> exists z', consume_trace initial_oracle z' t.
+  Proof.
+    intros.
+    eapply safety_trace in H as (b & q & m' & ? & ? & Hsafe); eauto.
+    exists b, q, m'; split; auto; split; auto.
+    intro n; destruct (Hsafe n) as [traces Hsafen].
+    exists traces; split; auto.
+    intros; eapply trace_correct; eauto.
+  Qed.
+
+End ext_trace.
 
 Require Import VST.progs.io_dry.
 Require Import VST.progs.io_os_connection.
@@ -125,9 +337,11 @@ Context {Hclen : ConsoleLen} {Horacle : SerialOracle}.
 
 Definition IO_inj_mem m s := st_mem s = m /\ valid_state s. (* stub *)
 
-Instance Espec : OracleKind := io_specs.IO_Espec ext_link.
+Instance IO_Espec : OracleKind := io_specs.IO_Espec ext_link.
 
-Theorem IO_OS_safety:
+Definition lift_IO_event e := existT (fun X => (io_specs.IO_event X * X)%type) (trace_event_rtype e) (io_event_of_io_tevent e).
+
+Theorem IO_OS_soundness:
  forall {CS: compspecs} (initial_oracle: OK_ty) V G m,
    semax_prog_ext prog initial_oracle V G ->
    Genv.init_mem prog = Some m ->
@@ -135,11 +349,10 @@ Theorem IO_OS_safety:
      Genv.find_symbol (Genv.globalenv prog) (prog_main prog) = Some b /\
      initial_core  (cl_core_sem (globalenv prog))
          0 m q m' (Vptr b Ptrofs.zero) nil /\
-     forall n,
-      ext_safeN prog IO_ext_sem consume_trace IO_inj_mem st_mem
-           n initial_oracle q m'.
+   forall n, exists traces, ext_safeN_trace(J := OK_spec) prog IO_ext_sem IO_inj_mem st_mem lift_IO_event n traces initial_oracle q m' /\
+     forall t, In _ traces t -> exists z', consume_trace initial_oracle z' t.
 Proof.
-  intros; eapply OS_safety with (dryspec := io_dry_spec ext_link); eauto.
+  intros; eapply OS_soundness with (dryspec := io_dry_spec ext_link); eauto.
   - unfold IO_ext_sem; intros; simpl in *.
     destruct H2 as [? Hvalid]; subst.
     if_tac; [|if_tac; [|contradiction]].
